\documentclass[12pt]{article}
\input{../preamble}

\title{Assignment 3}
\setcounter{assignment}{3}
\author{Naman Mishra}
\date{25 January, 2024}

\begin{document}
\maketitle
\begin{problem} \end{problem}

\begin{solution}[A]
    Let $b > 1$ and $n > 0$.
    Let $B = \set{t \in \R : t > 0, t^n < b}$.
    Since $b > 1$, $b^n > b$.
    Moreover, since $x < y \implies x^n < y^n$, where $x$ and $y$ are
    positive, we have that $b$ is an upper bound for $B$.
    By definition of $B$, $1 \in B$.
    Thus $B$ has a supremum.

    Now if $u < v$ are positive real numbers, then $u^n < v^n$.
    Thus there can be at most one positive $t$ such that $t^n = b$.

    We now show that $(\sup B)^n = b$.
    For this we show that $B$ has no largest element.
    For any $u \in B$, let $\delta = \min\set{\frac{b-u^n}{2^n}, 1}$.
    Then \begin{align*}
    (u(1 + \delta))^n
        &= u^n (1 + n \delta + \dots + \delta^n) \\
        &= u^n + \delta \sum_{j=1}^{n} \binom{n}{j} \\
        &< u^n + 2^n \delta \\
        &\le u^n + b - u^n \\
        &= b
    \end{align*}
    Thus $u(1 + \delta)$ is an element of $B$ greater than $u$.

    This implies that $\sup B \notin B$.
    Now let $u = \sup B$ and suppose $u^n > b$.
    Let \begin{align*}
        v   &= u + \frac{u^n - b}{nb + u^{n-1}} \\
            &= \frac{nbu + b}{nb + u^{n-1}}
        \shortintertext{as before. Then $0 < v < u$ and}
        v^n - b
            &= \frac{(nbu + b)^n - b(nb + u^{n-1})^n}{(nb + u^{n-1})^n} \\
            &> \frac{(nbu + b)^n - (nbu + u^n)^n}{(nb + u^{n-1})^n} \\
            &> 0
    \end{align*}
    But since $x \mapsto x^n$ is 
\end{solution}

\end{document}
